A12Kernel/Conformance.lean
@@ -68,6 +68,7 @@ import A12Kernel.Conformance.FullDateApplication
 import A12Kernel.Conformance.DateTimeApplication
 import A12Kernel.Conformance.FullDateComputationResult
 import A12Kernel.Conformance.DateTimeComputationResult
+import A12Kernel.Conformance.DateRangeSourceTargetState
 import A12Kernel.Conformance.FullDateComputation
 import A12Kernel.Conformance.DateTimeComputation
 import A12Kernel.Conformance.CorrelationElaboration
